src/lang.v
@@ -1,7 +1,7 @@
 Require Import base.
 Require Import PathToSubtree.
 From Stdlib Require Import PArith.
-From stdpp Require Import base.
+From stdpp Require Import gmap pmap.
 
 Definition var := positive.
 
@@ -22,10 +22,6 @@ Variant proj :=
    Do not mix paths (syntactical constructs of the language) with vpaths and spaths (the
    canonical way to denotes sub-values in a value of the state.)
 *)
-(* TODO: notation *)
-Definition path := list proj.
-Definition place : Set := var * path.
-
 Inductive type :=
 | TInt
 | TRef (t : type)
@@ -44,43 +40,123 @@ Proof.
       (left ; reflexivity) || (right ; intros contra ; congruence).
 Qed.
 
+(* TODO: notation *)
+Definition path := list proj.
+Definition place : Set := var * path * type.
+
+Variant const :=
+| IntConst (n : nat) (* TODO: use Aeneas integer types? *)
+| BoolConst (b : bool).
+
 Variant operand :=
-| IntConst (t : type) (n : nat) (* TODO: use Aeneas integer types? *)
-| Move (t : type) (p : place)
-| Copy (t : type) (p : place).
+| Const (c : const)
+| Move (p : place)
+| Copy (p : place).
+
+Variant BinOp :=
+| BAdd
+| BLe.
 
 Variant rvalue :=
-| Just (t : type) (op : operand)
-| BinOp (t : type) (op_l : operand) (op_r : operand)
-| BorrowMut (t : type) (p : place)
-| Pair (t : type) (op_l : operand) (op_r : operand).
+| Use (op : operand)
+| BinaryOp (b : BinOp) (op_l : operand) (op_r : operand)
+| BorrowMut (p : place).
 
 Inductive statement :=
 | Nop
 | Assign (p : place) (rv : rvalue)
 | Seq (stmt_0 : statement) (stmt_1 : statement)
-| Panic.
+(* Note: this should be generalized to match any enumerations, as booleans should only be a
+ * particular type of enumeration. *)
+| SwitchBool (op : operand) (stmt_if : statement) (stmt_else : statement)
+| Loop (body : statement)
+| Panic
+| Break
+| Continue
+.
 
-
-(* TODO: notation scope. *)
-Notation "s0 ;; s1" := (Seq s0 s1)
-  (at level 100, s1 at level 200, only parsing, right associativity).
-Notation "'&mut' p : t" := (BorrowMut t p) (at level 85, p at next level, t at next level).
-Notation "'INT' p" := (IntConst TInt p) (at level 80, p at next level).
-Notation "'ASSIGN' p <- rv" := (Assign p rv) (at level 90).
-
-Local Open Scope positive_scope.
-Check (&mut (1, nil) : TRef TInt) : rvalue.
-Check (ASSIGN (2, nil) <- &mut (1, nil) : TRef TInt).
-Check (ASSIGN (1, nil) <- Just TInt (INT 3)).
-Check (ASSIGN (1, nil) <- Just TInt (INT 3) ;;
-       ((ASSIGN (2, nil) <- &mut (1, nil) : TRef TInt) ;; Panic)).
 
 (* These definitions are not part of the grammar, but they are common for several (all?) semantics of the LLBC. *)
-Definition loan_id := nat.
+Definition loan_id := positive.
 
 Variant permission := Imm | Mut | Mov.
 
-Variant statement_result : Set :=
+(* TODO: notation scope. *)
+(* TODO: this notation conflicts with a stdpp notation. *)
+Notation "s0 ;; s1" := (Seq s0 s1)
+  (at level 100, s1 at level 200, only parsing, right associativity).
+Notation "&mut p" := (BorrowMut p) (at level 80).
+Notation "'ASSIGN' p <- rv" := (Assign p rv) (at level 90).
+Notation "'IF'  op  {{  stmt_if  }}  'ELSE'  {{  stmt_else  }}" := (SwitchBool op stmt_if stmt_else)
+  (at level 90).
+Notation "'LOOP'  {{  body  }}" := (Loop body) (at level 90).
+
+Reserved Notation "'loan^m' ( l )" (at level 0).
+Reserved Notation "'loan^m' ( ty , l )" (at level 0).
+Reserved Notation "'borrow^m' ( l , v )" (at level 0, l at next level, v at next level).
+Reserved Notation "'loc' ( l , v )" (at level 0, l at next level, v at next level).
+Reserved Notation "'ptr' ( l )" (at level 0).
+
+Reserved Notation "'nbot'" (at level 0).
+Reserved Notation "'nloan^m'( ty , l )" (at level 0).
+Reserved Notation "'nloan^m'( l )" (at level 0).
+Reserved Notation "'nborrow^m' ( l )" (at level 0, l at next level).
+Reserved Notation "'nloc' ( l )" (at level 0, l at next level).
+Reserved Notation "'nptr' ( l )" (at level 0).
+
+(* TODO: reserved notation for place evaluation. *)
+Reserved Notation "S  |-{op}  op  =>  r" (at level 60).
+Reserved Notation "S  |-{rv}  rv  =>  r" (at level 50).
+Reserved Notation "S  |-{stmt}  stmt  ~>{ n }  B" (at level 50).
+Global Reserved Notation "S  |-#  stmt  ~>  B" (at level 50).
+
+(** LLBC is a langage with non-local control-flow management, with the << break >>, << continue >>, << panic >> and << return >> keywords. As such, statements yield a *control-flow token*, that determines the continuation of the computation. *)
+Variant flow_token : Set :=
 | rPanic
-| rUnit. (* Panicless termination. *)
+| rUnit (* Panicless termination. TODO: rename. *)
+| rBreak
+| rContinue
+.
+
+(** Control-flow tags can be keys for [gmap]. *)
+Global Instance flow_token_eq_dec : EqDecision flow_token.
+Proof. unfold EqDecision, Decision. decide equality. Qed.
+
+Definition encode_flow_token r :=
+  match r with
+  | rPanic => 1%positive
+  | rUnit => 2%positive
+  | rBreak => 3%positive
+  | rContinue => 4%positive
+  end.
+
+Definition decode_flow_token r :=
+  match r with
+  | 1%positive => Some rPanic
+  | 2%positive => Some rUnit
+  | 3%positive => Some rBreak
+  | 4%positive => Some rContinue
+  | _ => None
+  end.
+
+Program Global Instance flow_token_countable : Countable flow_token := {
+  encode := encode_flow_token;
+  decode := decode_flow_token
+}.
+Next Obligation. intros [ ]; reflexivity. Qed.
+
+(** If the execution of the loop body ends on a token [r <> rContinue], computes the tag of the state after the loop. *)
+Definition end_loop_tag r : option flow_token :=
+  match r with
+  (** If the loop ends on a break, the program continues as usual. *)
+  | rBreak => Some rUnit
+  (** Panics are propagated through the loop. *)
+  | rPanic => Some rPanic
+  (** Note that [end_loop_tag] is not defined for [rContinue] and [rUnit].
+     - If the body ends on [rContinue], it loops back.
+     - If the body ends on [rUnit], the behavior is not defined, the program gets stuck. *)
+  | _ => None
+  end.
+
+Lemma partial_inj_end_loop_tag : partial_inj end_loop_tag.
+Proof. intros r0 (? & H) r1. destruct r0; destruct r1; easy. Qed.
